src/proofs/no_slashable_attestations/supporting_lemmas/dv_next_invs_8_18.dfy
@@ -285,7 +285,7 @@ module DV_Next_Invs_8_18
         }   
     }  
 
-    lemma lemma_inv18_dv_next(
+    lemma lemma_inv_queued_att_duty_is_higher_than_latest_served_att_duty_dv_next(
         dv: DVState,
         event: DV.Event,
         dv': DVState
@@ -299,8 +299,8 @@ module DV_Next_Invs_8_18
     requires inv7(dv)
     requires inv13(dv)  
     requires inv17(dv)
-    requires inv18(dv)
-    ensures inv18(dv')
+    requires inv_queued_att_duty_is_higher_than_latest_served_att_duty(dv)
+    ensures inv_queued_att_duty_is_higher_than_latest_served_att_duty(dv')
     {        
         match event 
         {
@@ -314,13 +314,13 @@ module DV_Next_Invs_8_18
                         
                         assert inv14_body(dvc, attestation_duty); 
                         assert inv15_body(dvc, attestation_duty);                                             
-                        lemma_inv18_f_serve_attestation_duty(dvc, attestation_duty, dvc');    
+                        lemma_inv_queued_att_duty_is_higher_than_latest_served_att_duty_f_serve_attestation_duty(dvc, attestation_duty, dvc');    
                         
                     case AttConsensusDecided(id, decided_attestation_data) => 
-                        lemma_inv18_f_att_consensus_decided(dvc, id, decided_attestation_data, dvc');                                                
+                        lemma_inv_queued_att_duty_is_higher_than_latest_served_att_duty_f_att_consensus_decided(dvc, id, decided_attestation_data, dvc');                                                
                         
                     case ReceivedAttestationShare(attestation_share) =>                         
-                        lemma_inv18_f_listen_for_attestation_shares(dvc, attestation_share, dvc');                        
+                        lemma_inv_queued_att_duty_is_higher_than_latest_served_att_duty_f_listen_for_attestation_shares(dvc, attestation_share, dvc');                        
                        
                     case ImportedNewBlock(block) =>                     
                         var dvc_mod := add_block_to_bn(dvc, block);
@@ -328,35 +328,35 @@ module DV_Next_Invs_8_18
                         assert inv5_body(dvc_mod);
                         lemma_inv17_add_block_to_bn(dvc, block, dvc_mod);
                         assert inv17_body(dvc_mod);
-                        lemma_inv18_add_block_to_bn(dvc, block, dvc_mod);
-                        assert inv18_body(dvc_mod);
+                        lemma_inv_queued_att_duty_is_higher_than_latest_served_att_duty_add_block_to_bn(dvc, block, dvc_mod);
+                        assert inv_queued_att_duty_is_higher_than_latest_served_att_duty_body(dvc_mod);
 
-                        lemma_inv18_f_listen_for_new_imported_blocks(dvc_mod, block, dvc');                        
-                        assert inv18_body(dvc');
+                        lemma_inv_queued_att_duty_is_higher_than_latest_served_att_duty_f_listen_for_new_imported_blocks(dvc_mod, block, dvc');                        
+                        assert inv_queued_att_duty_is_higher_than_latest_served_att_duty_body(dvc');
                     
                     case ResendAttestationShares =>                                                                                      
 
                     case NoEvent => 
                         
                 }
-                assert inv18_body(dvc');
+                assert inv_queued_att_duty_is_higher_than_latest_served_att_duty_body(dvc');
 
                 forall n | n in dv'.honest_nodes_states.Keys 
-                ensures inv18_body(dv'.honest_nodes_states[n]);
+                ensures inv_queued_att_duty_is_higher_than_latest_served_att_duty_body(dv'.honest_nodes_states[n]);
                 {
                     if n != node 
                     {
                         assert dv.honest_nodes_states[n] == dv'.honest_nodes_states[n];
-                        assert inv18_body(dv'.honest_nodes_states[n]);
+                        assert inv_queued_att_duty_is_higher_than_latest_served_att_duty_body(dv'.honest_nodes_states[n]);
                     }
                 }                
                 
             case AdeversaryTakingStep(node, new_attestation_share_sent, messagesReceivedByTheNode) =>
                 forall n | n in dv'.honest_nodes_states.Keys 
-                ensures inv18_body(dv'.honest_nodes_states[n]);
+                ensures inv_queued_att_duty_is_higher_than_latest_served_att_duty_body(dv'.honest_nodes_states[n]);
                 {
                     assert dv.honest_nodes_states[n] == dv'.honest_nodes_states[n];
-                    assert inv18_body(dv'.honest_nodes_states[n]);
+                    assert inv_queued_att_duty_is_higher_than_latest_served_att_duty_body(dv'.honest_nodes_states[n]);
                 }   
                 
         }   
