src/proofs/no_slashable_attestations/supporting_lemmas/fnc_invs_1_26.dfy
@@ -1826,7 +1826,7 @@ module Fnc_Invs_1_26
         lemma_inv17_f_check_for_next_queued_duty(process_mod, process');        
     } 
 
-    lemma lemma_inv18_f_listen_for_attestation_shares(
+    lemma lemma_inv_queued_att_duty_is_higher_than_latest_served_att_duty_f_listen_for_attestation_shares(
         process: DVCState,
         attestation_share: AttestationShare,
         process': DVCState
@@ -1835,22 +1835,22 @@ module Fnc_Invs_1_26
     requires process' == f_listen_for_attestation_shares(process, attestation_share).state    
     requires inv5_body(process)
     requires inv17_body(process)
-    requires inv18_body(process)
-    ensures inv18_body(process')
+    requires inv_queued_att_duty_is_higher_than_latest_served_att_duty_body(process)
+    ensures inv_queued_att_duty_is_higher_than_latest_served_att_duty_body(process')
     {}
 
-    lemma lemma_inv18_f_resend_attestation_share(
+    lemma lemma_inv_queued_att_duty_is_higher_than_latest_served_att_duty_f_resend_attestation_share(
         process: DVCState,
         process': DVCState)
     requires f_resend_attestation_share.requires(process)
     requires process' == f_resend_attestation_share(process).state    
     requires inv5_body(process)
     requires inv17_body(process)
-    requires inv18_body(process)
-    ensures inv18_body(process')
+    requires inv_queued_att_duty_is_higher_than_latest_served_att_duty_body(process)
+    ensures inv_queued_att_duty_is_higher_than_latest_served_att_duty_body(process')
     { }  
     
-    lemma lemma_inv18_add_block_to_bn(
+    lemma lemma_inv_queued_att_duty_is_higher_than_latest_served_att_duty_add_block_to_bn(
         s: DVCState,
         block: BeaconBlock,
         s': DVCState 
@@ -1859,22 +1859,22 @@ module Fnc_Invs_1_26
     requires s' == add_block_to_bn(s, block)
     requires inv5_body(s)
     requires inv17_body(s)
-    requires inv18_body(s)
-    ensures inv18_body(s')
+    requires inv_queued_att_duty_is_higher_than_latest_served_att_duty_body(s)
+    ensures inv_queued_att_duty_is_higher_than_latest_served_att_duty_body(s')
     { }
 
-    lemma lemma_inv18_f_start_next_duty(process: DVCState, attestation_duty: AttestationDuty, process': DVCState)
+    lemma lemma_inv_queued_att_duty_is_higher_than_latest_served_att_duty_f_start_next_duty(process: DVCState, attestation_duty: AttestationDuty, process': DVCState)
     requires f_start_next_duty.requires(process, attestation_duty)
     requires process' == f_start_next_duty(process, attestation_duty).state   
     requires forall queued_duty: AttestationDuty | queued_duty in process.attestation_duties_queue ::
                         attestation_duty.slot < queued_duty.slot     
     requires inv5_body(process)
     requires inv17_body(process)                        
-    requires inv18_body(process)
-    ensures inv18_body(process')
+    requires inv_queued_att_duty_is_higher_than_latest_served_att_duty_body(process)
+    ensures inv_queued_att_duty_is_higher_than_latest_served_att_duty_body(process')
     { } 
 
-    lemma lemma_inv18_f_check_for_next_queued_duty(
+    lemma lemma_inv_queued_att_duty_is_higher_than_latest_served_att_duty_f_check_for_next_queued_duty(
         process: DVCState,
         process': DVCState
     )
@@ -1882,9 +1882,9 @@ module Fnc_Invs_1_26
     requires process' == f_check_for_next_queued_duty(process).state    
     requires inv5_body(process)
     requires inv17_body(process)
-    requires inv18_body(process)
+    requires inv_queued_att_duty_is_higher_than_latest_served_att_duty_body(process)
     ensures inv17_body(process')
-    ensures inv18_body(process')
+    ensures inv_queued_att_duty_is_higher_than_latest_served_att_duty_body(process')
     decreases process.attestation_duties_queue
     {
         if  && process.attestation_duties_queue != [] 
@@ -1906,7 +1906,7 @@ module Fnc_Invs_1_26
                             new_attestation_slashing_db
                         )                        
                     );
-                    lemma_inv18_f_check_for_next_queued_duty(process_mod, process');
+                    lemma_inv_queued_att_duty_is_higher_than_latest_served_att_duty_f_check_for_next_queued_duty(process_mod, process');
                 }
                 else
                 { 
@@ -1920,9 +1920,9 @@ module Fnc_Invs_1_26
                                     next_duty.slot <= queued_duty.slot;
 
 
-                    assert inv18_body(process_mod);
+                    assert inv_queued_att_duty_is_higher_than_latest_served_att_duty_body(process_mod);
 
-                    lemma_inv18_f_start_next_duty(process_mod, next_duty, process');
+                    lemma_inv_queued_att_duty_is_higher_than_latest_served_att_duty_f_start_next_duty(process_mod, next_duty, process');
                 }
         }
         else
@@ -1931,7 +1931,7 @@ module Fnc_Invs_1_26
         }
     }
 
-    lemma lemma_inv18_f_serve_attestation_duty(
+    lemma lemma_inv_queued_att_duty_is_higher_than_latest_served_att_duty_f_serve_attestation_duty(
         process: DVCState,
         attestation_duty: AttestationDuty,
         process': DVCState
@@ -1942,10 +1942,10 @@ module Fnc_Invs_1_26
     requires inv12_body(process, attestation_duty)  
     requires inv15_body(process, attestation_duty)  
     requires inv17_body(process)
-    requires inv18_body(process)
+    requires inv_queued_att_duty_is_higher_than_latest_served_att_duty_body(process)
     requires forall queued_duty: AttestationDuty | queued_duty in process.attestation_duties_queue ::
                         queued_duty.slot < attestation_duty.slot
-    ensures inv18_body(process')
+    ensures inv_queued_att_duty_is_higher_than_latest_served_att_duty_body(process')
     {
         var process_mod := process.(
                 attestation_duties_queue := process.attestation_duties_queue + [attestation_duty],
@@ -1960,19 +1960,19 @@ module Fnc_Invs_1_26
             assert process.latest_attestation_duty.safe_get().slot < attestation_duty.slot;
             assert process_mod.latest_attestation_duty.safe_get().slot < attestation_duty.slot;
             assert inv17_body(process_mod);      
-            assert inv18_body(process_mod);      
+            assert inv_queued_att_duty_is_higher_than_latest_served_att_duty_body(process_mod);      
         }
         else 
         {
             assert !process_mod.latest_attestation_duty.isPresent();
             assert inv17_body(process_mod);      
-            assert inv18_body(process_mod);      
+            assert inv_queued_att_duty_is_higher_than_latest_served_att_duty_body(process_mod);      
         }
         
-        lemma_inv18_f_check_for_next_queued_duty(process_mod, process');        
+        lemma_inv_queued_att_duty_is_higher_than_latest_served_att_duty_f_check_for_next_queued_duty(process_mod, process');        
     } 
 
-    lemma lemma_inv18_f_listen_for_new_imported_blocks(
+    lemma lemma_inv_queued_att_duty_is_higher_than_latest_served_att_duty_f_listen_for_new_imported_blocks(
         process: DVCState,
         block: BeaconBlock,
         process': DVCState
@@ -1981,8 +1981,8 @@ module Fnc_Invs_1_26
     requires process' == f_listen_for_new_imported_blocks(process, block).state    
     requires inv5_body(process)
     requires inv17_body(process)
-    requires inv18_body(process)
-    ensures inv18_body(process')
+    requires inv_queued_att_duty_is_higher_than_latest_served_att_duty_body(process)
+    ensures inv_queued_att_duty_is_higher_than_latest_served_att_duty_body(process')
     {
         var new_consensus_instances_already_decided := f_listen_for_new_imported_blocks_helper_1(process, block);
 
@@ -2004,7 +2004,7 @@ module Fnc_Invs_1_26
 
         assert inv5_body(process);
         assert inv17_body(process);
-        assert inv18_body(process);
+        assert inv_queued_att_duty_is_higher_than_latest_served_att_duty_body(process);
                     
 
         if process.current_attestation_duty.isPresent() && process.current_attestation_duty.safe_get().slot in att_consensus_instances_already_decided
@@ -2022,17 +2022,17 @@ module Fnc_Invs_1_26
 
             assert inv5_body(process);
             assert inv17_body(process);
-            assert inv18_body(process);
+            assert inv_queued_att_duty_is_higher_than_latest_served_att_duty_body(process);
 
-            lemma_inv18_f_check_for_next_queued_duty(process, process');
+            lemma_inv_queued_att_duty_is_higher_than_latest_served_att_duty_f_check_for_next_queued_duty(process, process');
         }
         else
         {               
-            assert inv18_body(process);
+            assert inv_queued_att_duty_is_higher_than_latest_served_att_duty_body(process);
         }
     } 
 
-    lemma lemma_inv18_f_att_consensus_decided(
+    lemma lemma_inv_queued_att_duty_is_higher_than_latest_served_att_duty_f_att_consensus_decided(
         process: DVCState,
         id: Slot,
         decided_attestation_data: AttestationData, 
@@ -2042,8 +2042,8 @@ module Fnc_Invs_1_26
     requires process' == f_att_consensus_decided(process, id, decided_attestation_data).state     
     requires inv5_body(process)
     requires inv17_body(process)
-    requires inv18_body(process)
-    ensures inv18_body(process')
+    requires inv_queued_att_duty_is_higher_than_latest_served_att_duty_body(process)
+    ensures inv_queued_att_duty_is_higher_than_latest_served_att_duty_body(process')
     {
         
         if  || !process.current_attestation_duty.isPresent()
@@ -2078,11 +2078,11 @@ module Fnc_Invs_1_26
 
         assert inv5_body(process);
         assert inv17_body(process);
-        assert inv18_body(process);
+        assert inv_queued_att_duty_is_higher_than_latest_served_att_duty_body(process);
 
         var ret_check_for_next_queued_duty := f_check_for_next_queued_duty(process);
         
-        lemma_inv18_f_check_for_next_queued_duty(process, ret_check_for_next_queued_duty.state);
+        lemma_inv_queued_att_duty_is_higher_than_latest_served_att_duty_f_check_for_next_queued_duty(process, ret_check_for_next_queued_duty.state);
 
         assert process' == ret_check_for_next_queued_duty.state;        
     }  
@@ -2333,7 +2333,7 @@ module Fnc_Invs_1_26
     requires f_check_for_next_queued_duty.requires(process)
     requires process' == f_check_for_next_queued_duty(process).state        
     requires inv17_body(process)
-    requires inv18_body(process)
+    requires inv_queued_att_duty_is_higher_than_latest_served_att_duty_body(process)
     requires inv_no_active_consensus_instance_before_receiving_att_duty_body(process)
     requires inv_slot_of_active_consensus_instance_is_lower_than_slot_of_latest_served_att_duty_body(process)
     ensures inv_slot_of_active_consensus_instance_is_lower_than_slot_of_latest_served_att_duty_body(process')
@@ -2360,7 +2360,7 @@ module Fnc_Invs_1_26
                     );
 
                     assert inv17_body(process_mod);
-                    assert inv18_body(process_mod);
+                    assert inv_queued_att_duty_is_higher_than_latest_served_att_duty_body(process_mod);
                     assert inv_slot_of_active_consensus_instance_is_lower_than_slot_of_latest_served_att_duty_body(process_mod);
                 }
                 else
@@ -2372,7 +2372,7 @@ module Fnc_Invs_1_26
                     if process_mod.latest_attestation_duty.isPresent()
                     {
                         assert inv17_body(process_mod);
-                        assert inv18_body(process_mod);
+                        assert inv_queued_att_duty_is_higher_than_latest_served_att_duty_body(process_mod);
                         assert inv_slot_of_active_consensus_instance_is_lower_than_slot_of_latest_served_att_duty_body(process_mod);
 
                         assert  process_mod.latest_attestation_duty.isPresent()
@@ -2446,7 +2446,7 @@ module Fnc_Invs_1_26
     requires inv7_body(process)
     requires inv14_body(process, attestation_duty)
     requires inv17_body(process)
-    requires inv18_body(process)
+    requires inv_queued_att_duty_is_higher_than_latest_served_att_duty_body(process)
     requires inv_no_active_consensus_instance_before_receiving_att_duty_body(process)    
     requires inv_slot_of_active_consensus_instance_is_lower_than_slot_of_latest_served_att_duty_body(process)
     ensures inv_slot_of_active_consensus_instance_is_lower_than_slot_of_latest_served_att_duty_body(process')
@@ -2459,7 +2459,7 @@ module Fnc_Invs_1_26
         assert inv5_body(process_mod);
         assert inv7_body(process_mod);
         assert inv17_body(process_mod);                        
-        assert inv18_body(process_mod);         
+        assert inv_queued_att_duty_is_higher_than_latest_served_att_duty_body(process_mod);         
         assert inv_no_active_consensus_instance_before_receiving_att_duty_body(process_mod);         
         assert inv_slot_of_active_consensus_instance_is_lower_than_slot_of_latest_served_att_duty_body(process_mod);
         
@@ -2474,7 +2474,7 @@ module Fnc_Invs_1_26
     requires f_listen_for_new_imported_blocks.requires(process, block)
     requires process' == f_listen_for_new_imported_blocks(process, block).state        
     requires inv17_body(process)
-    requires inv18_body(process)
+    requires inv_queued_att_duty_is_higher_than_latest_served_att_duty_body(process)
     requires inv_no_active_consensus_instance_before_receiving_att_duty_body(process)
     requires inv_slot_of_active_consensus_instance_is_lower_than_slot_of_latest_served_att_duty_body(process)
     ensures inv_slot_of_active_consensus_instance_is_lower_than_slot_of_latest_served_att_duty_body(process')
@@ -2498,7 +2498,7 @@ module Fnc_Invs_1_26
                 );    
         
         assert inv17_body(process_mod);
-        assert inv18_body(process_mod);
+        assert inv_queued_att_duty_is_higher_than_latest_served_att_duty_body(process_mod);
         assert inv_no_active_consensus_instance_before_receiving_att_duty_body(process_mod);
         assert inv_slot_of_active_consensus_instance_is_lower_than_slot_of_latest_served_att_duty_body(process_mod);
 
@@ -2516,7 +2516,7 @@ module Fnc_Invs_1_26
             );
             
             assert inv17_body(temp_process);
-            assert inv18_body(temp_process);
+            assert inv_queued_att_duty_is_higher_than_latest_served_att_duty_body(temp_process);
             assert inv_no_active_consensus_instance_before_receiving_att_duty_body(temp_process);
             assert inv_slot_of_active_consensus_instance_is_lower_than_slot_of_latest_served_att_duty_body(temp_process);
 
@@ -2539,7 +2539,7 @@ module Fnc_Invs_1_26
     requires f_att_consensus_decided.requires(process, id, decided_attestation_data)
     requires process' == f_att_consensus_decided(process, id, decided_attestation_data).state         
     requires inv17_body(process)
-    requires inv18_body(process)
+    requires inv_queued_att_duty_is_higher_than_latest_served_att_duty_body(process)
     requires inv_no_active_consensus_instance_before_receiving_att_duty_body(process)
     requires inv_slot_of_active_consensus_instance_is_lower_than_slot_of_latest_served_att_duty_body(process)
     ensures inv_slot_of_active_consensus_instance_is_lower_than_slot_of_latest_served_att_duty_body(process')
@@ -2576,7 +2576,7 @@ module Fnc_Invs_1_26
             );
 
         assert inv17_body(process_mod);
-        assert inv18_body(process_mod);
+        assert inv_queued_att_duty_is_higher_than_latest_served_att_duty_body(process_mod);
         assert inv_no_active_consensus_instance_before_receiving_att_duty_body(process_mod);
         assert inv_slot_of_active_consensus_instance_is_lower_than_slot_of_latest_served_att_duty_body(process_mod);
 
