src/proofs/no_slashable_attestations/supporting_lemmas/proofs_ind_inv.dfy
@@ -75,12 +75,12 @@ module Proofs_DV_Ind_Inv
         &&  inv13(dv)      
         &&  inv16(dv)  
         &&  inv17(dv)  
-        &&  inv18(dv)  
+        &&  inv_queued_att_duty_is_higher_than_latest_served_att_duty(dv)  
     }
     
     predicate invs_19_26(dv: DVState)       
     {        
-        &&  inv19(dv)           
+        &&  inv_no_duplicated_att_duties(dv)           
         &&  inv_every_att_duty_before_dvn_att_index_was_delivered(dv) 
         &&  inv_no_active_consensus_instance_before_receiving_att_duty(dv)      
         &&  inv_slot_of_active_consensus_instance_is_lower_than_slot_of_latest_served_att_duty(dv)  
@@ -160,7 +160,7 @@ module Proofs_DV_Ind_Inv
         lemma_inv13_dv_next(dv, e, dv');                
         // lemma_inv16_dv_next(dv, e, dv');
         // lemma_inv17_dv_next(dv, e, dv');
-        // lemma_inv18_dv_next(dv, e, dv');
+        // lemma_inv_queued_att_duty_is_higher_than_latest_served_att_duty_dv_next(dv, e, dv');
     }
 
     lemma lemma_ind_inv_dv_next_invs_8_18_helper_2(dv: DVState, e: DV.Event, dv': DVState)       
@@ -169,11 +169,11 @@ module Proofs_DV_Ind_Inv
     requires ind_inv(dv)
     ensures inv16(dv')
     ensures inv17(dv')
-    ensures inv18(dv')
+    ensures inv_queued_att_duty_is_higher_than_latest_served_att_duty(dv')
     {
         lemma_inv16_dv_next(dv, e, dv');
         lemma_inv17_dv_next(dv, e, dv');
-        lemma_inv18_dv_next(dv, e, dv');
+        lemma_inv_queued_att_duty_is_higher_than_latest_served_att_duty_dv_next(dv, e, dv');
     }
 
     lemma lemma_ind_inv_dv_next_invs_8_18(dv: DVState, e: DV.Event, dv': DVState)       
@@ -190,12 +190,12 @@ module Proofs_DV_Ind_Inv
     requires DV.NextEventPreCond(dv, e)
     requires DV.NextEvent(dv, e, dv')  
     requires ind_inv(dv)
-    ensures inv19(dv')        
+    ensures inv_no_duplicated_att_duties(dv')        
     ensures concl_unchanged_dvn_seq_of_att_duties(dv, dv')
     ensures inv_every_att_duty_before_dvn_att_index_was_delivered(dv')
     ensures inv_no_active_consensus_instance_before_receiving_att_duty(dv')
     {
-        lemma_inv19_dv_next(dv, e, dv');
+        lemma_inv_no_duplicated_att_duties_dv_next(dv, e, dv');
         lemma_concl_unchanged_dvn_seq_of_att_duties_dv_next(dv, e, dv');
         lemma_inv_every_att_duty_before_dvn_att_index_was_delivered_dv_next(dv, e, dv');        
         lemma_inv_no_active_consensus_instance_before_receiving_att_duty_dv_next(dv, e, dv');                
